extraction/theories/Erasure.v
@@ -506,9 +506,11 @@ erase_type Γ erΓ t wat tvars with inspect (reduce_term redβιζ Σ wfΣ Γ t 
       | et_view_sort _ := ret (tvars, TBox);
 
       | et_view_prod na A B with flag_of_type Γ A _ := {
-          (* For logical things just box and proceed *)
-        | Checked {| is_logical := true |} :=
-          '(tvars, bt) <- erase_type (Γ,, vass na A) (RelOther :: erΓ)%vector B _ tvars;;
+          (* For logical things, we add a type variable if it's an arity *)
+        | Checked {| is_logical := true ; is_arity := isar |} :=
+          let e := if isar then RelTypeVar (List.length tvars) else RelOther in
+          let tvars' := if isar then tvars ++ [na] else tvars in
+          '(tvars, bt) <- erase_type (Γ,, vass na A) (e :: erΓ)%vector B _ tvars';;
           ret (tvars, TArr TBox bt);
 
           (* If the type isn't an arity now, then it's a "normal" type like nat. *)
@@ -877,14 +879,15 @@ Program Definition erase_ind_body
 
   let '(Γ; erΓ) := arities_contexts mind (P.ind_bodies mib) in
 
+  let ind_params := firstn (P.ind_npars mib) oib_tvars in
+  let the_rest := skipn (P.ind_npars mib) oib_tvars in
+  (* we filter out non-arities from the inductive parameters since non-arities
+     will not be type variables *)
+  let ind_params_arities_only := filter tvar_is_arity ind_params in
   (* We map type vars in constructors to type vars in the inductive parameters.
-     Thus, we only allow the constructor this many type vars. *)
+     Thus, we only allow the constructor this many type vars *)
   let num_tvars_in_params :=
-      List.length
-        (filter
-           (fun tvar => negb (tvar_is_logical tvar) && tvar_is_sort tvar)
-           (firstn (P.ind_npars mib) oib_tvars)) in
-
+      List.length ind_params_arities_only in
   let erase_ind_ctor (p : (ident × P.term) × nat) (is_in : In p (P.ind_ctors oib)) :=
       let '((name, t), _) := p in
       '(ctor_tvars, bt) <- map_error (EraseCtorError name)
@@ -901,7 +904,7 @@ Program Definition erase_ind_body
   ctors <- monad_map_in (P.ind_ctors oib) erase_ind_ctor;;
 
   ret {| ind_name := P.ind_name oib;
-         ind_type_vars := oib_tvars;
+         ind_type_vars := ind_params_arities_only ++ the_rest;
          ind_ctors := ctors;
          ind_projs := [] (* todo *) |}.
 Next Obligation.
